

University of Nebraska-Lincoln

Digital Signal Processing: Quiz 1

August 29, 2025

Name: _____

Total Points: 10

1. (10 points) Consider the frequency response

$$H(e^{j\omega}) = \frac{1 + e^{-j\omega}}{3 - 2e^{-j\omega}}$$

Find the **real part** of $H(e^{j\omega})$ as a function of ω . **Note:** don't leave any j 's, i 's, $\sqrt{-1}$'s, etc.

Solution:

First, express all terms in terms of sines and cosines:

$$e^{-j\omega} = \cos \omega - j \sin \omega$$

$$1 + e^{-j\omega} = 1 + \cos \omega - j \sin \omega$$

$$3 - 2e^{-j\omega} = 3 - 2\cos \omega + j2\sin \omega$$

Let $A = 1 + \cos \omega$, $B = -\sin \omega$, $C = 3 - 2\cos \omega$, $D = 2\sin \omega$, so

$$H(e^{j\omega}) = \frac{A + jB}{C + jD}$$

Multiply numerator and denominator by the complex conjugate of the denominator:

$$\begin{aligned} & (C - jD) \\ H(e^{j\omega}) &= \frac{(A + jB)(C - jD)}{(C + jD)(C - jD)} \\ &= \frac{AC + BD + j(BC - AD)}{C^2 + D^2} \end{aligned}$$

The real part is:

$$\operatorname{Re}\{H(e^{j\omega})\} = \frac{AC + BD}{C^2 + D^2}$$

Substitute back:

$$AC = (1 + \cos \omega)(3 - 2\cos \omega) = 3 + 3\cos \omega - 2\cos \omega - 2\cos^2 \omega = 3 + \cos \omega - 2\cos^2 \omega$$

$$BD = (-\sin \omega)(2\sin \omega) = -2\sin^2 \omega$$

$$AC + BD = 3 + \cos \omega - 2\cos^2 \omega - 2\sin^2 \omega$$

Recall that $\sin^2 \omega + \cos^2 \omega = 1$, so:

$$-2\cos^2 \omega - 2\sin^2 \omega = -2(\cos^2 \omega + \sin^2 \omega) = -2$$

$$AC + BD = 3 + \cos \omega - 2 = 1 + \cos \omega$$

The denominator:

$$C^2 + D^2 = (3 - 2\cos \omega)^2 + [2\sin \omega]^2 = 9 - 12\cos \omega + 4\cos^2 \omega + 4\sin^2 \omega$$

$$= 9 - 12\cos \omega + 4(\cos^2 \omega + \sin^2 \omega)$$

$$= 9 - 12\cos \omega + 4(1) = 13 - 12\cos \omega$$

Therefore,

$$\boxed{\operatorname{Re}\{H(e^{j\omega})\} = \frac{1 + \cos \omega}{13 - 12\cos \omega}}$$